code/hash/Hacl.Hash.Definitions.fst
@@ -92,15 +92,7 @@ let as_seq (#i:impl) (h:HS.mem) (s:state i) : GTot (words_state (get_alg i)) =
   match a with
   | MD5 | SHA1 | SHA3_256 -> B.as_seq h s
   | SHA2_224 | SHA2_256 | SHA2_384 | SHA2_512 ->
-      // The agile hash specification has no notion of vectorized words, so we
-      // "dereference" the single-element vector to obtain a vector of uint32s
-      // or uint64s
-      let s = B.as_seq h s in
-      let s = Seq.init 8 (fun j ->
-        let v = Seq.index s j in
-        let v = Lib.IntVector.vec_v #(Spec.Hash.Definitions.word_t a) #1 v in
-        Seq.index v 0 <: Spec.Hash.Definitions.word a) in
-      s
+      Seq.index Hacl.Spec.SHA2.Vec.(state_spec_v #a #M32 (B.as_seq h s)) 0
   | Blake2S -> Blake2.state_v #Spec.Blake2.Blake2S #(get_spec i) h s
   | Blake2B -> Blake2.state_v #Spec.Blake2.Blake2B #(get_spec i) h s
 
